feat: more generic definition for the equality

Garden/Plonky3/M.v
@@ -42,6 +42,16 @@ Module Default.
   }.
 End Default.
 
+Module Equal.
+  Class C (A : Set) : Type := {
+    t : A -> A -> Prop;
+  }.
+End Equal.
+
+Global Instance ZIsEqual : Equal.C Z := {
+  Equal.t := eq;
+}.
+
 Module Array.
   Record t {A : Set} {N : Z} : Set := {
     get : Z -> A;
@@ -101,10 +111,14 @@ Module Array.
   }.
 
   Module Eq.
-    Definition t {A : Set} {N : Z} (x y : t A N) : Prop :=
-      forall (i : Z), 0 <= i < N -> x.(get) i = y.(get) i.
+    Global Instance IsEqual (A : Set) (N : Z) `{Equal.C A} : Equal.C (t A N) := {
+      Equal.t (x y : t A N) :=
+        forall (i : Z),
+        0 <= i < N ->
+        Equal.t (x.(get) i) (y.(get) i);
+    }.
 
-    Axiom dec : forall {A : Set} {N : Z} (x y : Array.t A N), {t x y} + {~ t x y}.
+    Axiom dec : forall {N : Z} (x y : Array.t Z N), {Equal.t x y} + {~ Equal.t x y}.
   End Eq.
 End Array.
 
@@ -343,87 +357,6 @@ Global Instance IsMapMod_Array {p} `{Prime p} (A : Set) (N : Z) `{MapMod p A} :
   map_mod := Array.map map_mod;
 }.
 
-Module Limbs.
-  Definition of_bools {p} `{Prime p} (NB_LIMBS BITS_PER_LIMB : Z)
-      (a : Array.t Z (NB_LIMBS * BITS_PER_LIMB)) :
-      Array.t Z NB_LIMBS :=
-    {|
-      Array.get limb :=
-        let l : list nat :=
-          List.rev (
-            List.seq
-              (Z.to_nat (limb * BITS_PER_LIMB))%Z
-              (Z.to_nat (limb * BITS_PER_LIMB + BITS_PER_LIMB))%Z
-          ) in
-        Lists.List.fold_left (fun acc (z : nat) =>
-          let z : Z := Z.of_nat z in
-          BinOp.add (BinOp.mul 2 acc) (a.(Array.get) z)
-        ) l 0
-    |}.
-
-  Lemma from_of_bools_eq {p} `{Prime p} (NB_LIMBS BITS_PER_LIMB : Z)
-      (a : Array.t Z (NB_LIMBS * BITS_PER_LIMB))
-      (H_bools :
-        forall (z : Z),
-        0 <= z < NB_LIMBS * BITS_PER_LIMB ->
-        IsBool.t (a.(Array.get) z)
-      )
-      (limb : Z) :
-    0 <= limb < NB_LIMBS ->
-    UnOp.from ((of_bools NB_LIMBS BITS_PER_LIMB a).(Array.get) limb) =
-    (of_bools NB_LIMBS BITS_PER_LIMB a).(Array.get) limb.
-  Admitted.
-
-  Definition get_bit {NB_LIMBS : Z} (BITS_PER_LIMB : Z)
-      (a : Array.t Z NB_LIMBS)
-      (bit : Z) :
-      bool :=
-    let limb := bit / BITS_PER_LIMB in
-    let bit_in_limb := bit mod BITS_PER_LIMB in
-    let limb_value := a.(Array.get) limb in
-    Z.testbit limb_value bit_in_limb.
-
-  Lemma get_bit_of_bools_eq {p} `{Prime p} (NB_LIMBS BITS_PER_LIMB : Z)
-      (a : Array.t Z (NB_LIMBS * BITS_PER_LIMB))
-      (bit : Z)
-      (H_bools :
-        forall (z : Z),
-        0 <= z < NB_LIMBS * BITS_PER_LIMB ->
-        IsBool.t (a.(Array.get) z)
-      ) :
-    get_bit BITS_PER_LIMB (of_bools NB_LIMBS BITS_PER_LIMB a) bit =
-    Z.odd (a.(Array.get) bit).
-  Admitted.
-
-  Lemma get_bit_of_bools_eqs {p} `{Prime p} (NB_LIMBS BITS_PER_LIMB : Z)
-      (a_limbs : Array.t Z NB_LIMBS)
-      (a_bools : Array.t Z (NB_LIMBS * BITS_PER_LIMB))
-      (H_bools :
-        forall (z : Z),
-        0 <= z < NB_LIMBS * BITS_PER_LIMB ->
-        IsBool.t (a_bools.(Array.get) z)
-      )
-      (H_limbs :
-        forall (limb : Z),
-        0 <= limb < NB_LIMBS ->
-        a_limbs.(Array.get) limb =
-        UnOp.from ((of_bools NB_LIMBS BITS_PER_LIMB a_bools).(Array.get) limb)
-      ) :
-    0 <= NB_LIMBS ->
-    forall (bit : Z),
-    0 <= bit < NB_LIMBS * BITS_PER_LIMB ->
-    get_bit BITS_PER_LIMB a_limbs bit =
-    Z.odd (a_bools.(Array.get) bit).
-  Proof.
-    intros.
-    unfold get_bit.
-    rewrite H_limbs by nia.
-    rewrite <- get_bit_of_bools_eq by assumption.
-    rewrite from_of_bools_eq; trivial.
-    nia.
-  Qed.
-End Limbs.
-
 Ltac show_equality_modulo :=
   unfold
     UnOp.from,
@@ -637,6 +570,100 @@ Module FieldRewrite.
     | H : _ |- _ => rewrite_db field_rewrite in H
     end.
 End FieldRewrite.
+
+(** Utilities around the manipulation of limbs *)
+Module Limbs.
+  (** Convert an array of bools to an array of limbs. *)
+  Definition of_bools {p} `{Prime p} (NB_LIMBS BITS_PER_LIMB : Z)
+      (a : Array.t Z (NB_LIMBS * BITS_PER_LIMB)) :
+      Array.t Z NB_LIMBS :=
+    {|
+      Array.get limb :=
+        let l : list nat :=
+          List.rev (
+            List.seq
+              (Z.to_nat (limb * BITS_PER_LIMB))%Z
+              (Z.to_nat (limb * BITS_PER_LIMB + BITS_PER_LIMB))%Z
+          ) in
+        (* We sum all the bits times 2 to the n *)
+        Lists.List.fold_left (fun acc (z : nat) =>
+          let z : Z := Z.of_nat z in
+          (2 *F acc) +F a.[z]
+        ) l 0
+    |}.
+
+  (** We have taken the modulo of the result. *)
+  Lemma from_of_bools_eq {p} `{Prime p} (NB_LIMBS BITS_PER_LIMB : Z)
+      (a : Array.t Z (NB_LIMBS * BITS_PER_LIMB))
+      (H_bools :
+        forall (z : Z),
+        0 <= z < NB_LIMBS * BITS_PER_LIMB ->
+        IsBool.t a.[z]
+      )
+      (limb : Z)
+      (H_limb : 0 <= limb < NB_LIMBS) :
+    UnOp.from (of_bools NB_LIMBS BITS_PER_LIMB a).[limb] =
+    (of_bools NB_LIMBS BITS_PER_LIMB a).[limb].
+  Proof.
+    cbn.
+    set (l := List.rev _); clearbody l.
+    assert (H_acc : UnOp.from 0 = 0) by trivial; revert H_acc.
+    generalize 0 as acc.
+    induction l; cbn; trivial; intros.
+    apply IHl.
+    now FieldRewrite.run.
+  Qed.
+
+  (** Extract a single bit from an array of limbs. *)
+  Definition get_bit {NB_LIMBS : Z} (BITS_PER_LIMB : Z)
+      (a : Array.t Z NB_LIMBS)
+      (bit : Z) :
+      bool :=
+    let limb := bit / BITS_PER_LIMB in
+    let bit_in_limb := bit mod BITS_PER_LIMB in
+    let limb_value := a.(Array.get) limb in
+    Z.testbit limb_value bit_in_limb.
+
+  Lemma get_bit_of_bools_eq {p} `{Prime p} (NB_LIMBS BITS_PER_LIMB : Z)
+      (a : Array.t Z (NB_LIMBS * BITS_PER_LIMB))
+      (bit : Z)
+      (H_bools :
+        forall (z : Z),
+        0 <= z < NB_LIMBS * BITS_PER_LIMB ->
+        IsBool.t (a.(Array.get) z)
+      ) :
+    get_bit BITS_PER_LIMB (of_bools NB_LIMBS BITS_PER_LIMB a) bit =
+    Z.odd a.[bit].
+  Admitted.
+
+  Lemma get_bit_of_bools_eqs {p} `{Prime p} (NB_LIMBS BITS_PER_LIMB : Z)
+      (a_limbs : Array.t Z NB_LIMBS)
+      (a_bools : Array.t Z (NB_LIMBS * BITS_PER_LIMB))
+      (H_bools :
+        forall (z : Z),
+        0 <= z < NB_LIMBS * BITS_PER_LIMB ->
+        IsBool.t a_bools.[z]
+      )
+      (H_limbs :
+        forall (limb : Z),
+        0 <= limb < NB_LIMBS ->
+        a_limbs.[limb] =
+        UnOp.from (of_bools NB_LIMBS BITS_PER_LIMB a_bools).[limb]
+      ) :
+    0 <= NB_LIMBS ->
+    forall (bit : Z),
+    0 <= bit < NB_LIMBS * BITS_PER_LIMB ->
+    get_bit BITS_PER_LIMB a_limbs bit =
+    Z.odd (a_bools.(Array.get) bit).
+  Proof.
+    intros.
+    unfold get_bit.
+    rewrite H_limbs by nia.
+    rewrite <- get_bit_of_bools_eq by assumption.
+    rewrite from_of_bools_eq; trivial.
+    nia.
+  Qed.
+End Limbs.
 
 (** Rules to check if the contraints are what we expect, typically a unique possible value. *)
 Module Run.
@@ -951,7 +978,6 @@ Module Test_mod_inverse.
   Proof.
     reflexivity.
   Qed.
-
 
   Definition test2 : Z := mod_inverse 2 11. 
   Goal test2 = 6.
